starting on 1.3 interop

src/tls/test/test_client.ml
@@ -1,7 +1,10 @@
 (* Main driver for interop tests *)
 
 let _ =
-  if (Array.length Sys.argv <> 3) then
-     TestClient.main "openssl.org" 443
+  if (Array.length Sys.argv <> 4) then
+     print_string "Usage: ./client.out <1.2|1.3> <host> <port>\n"
   else 
-     TestClient.main Sys.argv.(1) (int_of_string Sys.argv.(2))
+     if (Sys.argv.(1) = "1.3") then
+        TestClient13.main Sys.argv.(2) (int_of_string Sys.argv.(3))
+     else 
+        TestClient.main Sys.argv.(2) (int_of_string Sys.argv.(3))
