src/tls/test/TestClient.fst
@@ -102,6 +102,8 @@ let decryptRecord_TLS12_AES_GCM_128_SHA256 rd ct cipher =
   let (Some d) = StatefulLHAE.decrypt #id #ad rd cipher in
   Content.repr id d
 
+(* We should use Content.mk_fragment |> Content.repr, not Record.makePacket *)
+(* Even better, we should move to TLS.send *)
 
 let sendHSRecord tcp pv log hs_msg = 
   let r = Record.makePacket Content.Handshake pv hs_msg in
@@ -197,30 +199,47 @@ let main host port =
   IO.print_string "===============================================\n Starting test TLS client...\n";
   let tcp = Platform.Tcp.connect host port in
   let log = empty_bytes in
-  let (ch,chb) = Handshake.prepareClientHello config None None in
+  
+(*
+  let st = Handshake.init Client ... in
+  Handhake.send_client_hello st;
+  let chb = Handshake.next_message st in
+*)
+
+
+  let (None,ch,chb) = Handshake.prepareClientHello config None None in
   let pv = ch.ch_protocol_version in 
   let kex = TLSConstants.Kex_ECDHE in
+
   IO.print_string "Sending ClientHello\n";
   let log = sendHSRecord tcp pv log chb in
+
   let ServerHello(sh),log = recvHSRecord tcp pv kex log in
   IO.print_string "Received ServerHello\n";
+
   let pv = sh.sh_protocol_version in
   let cs = sh.sh_cipher_suite in
   let CipherSuite kex sa ae = cs in
+
   let Certificate(sc),log = recvHSRecord tcp pv kex log in
   IO.print_string "Received ServerCertificate\n";
+
   let ServerKeyExchange(ske),log = recvHSRecord tcp pv kex log in
   IO.print_string "Received ServerKeyExchange\n";
+
   let ServerHelloDone,log = recvHSRecord tcp pv kex log in
   IO.print_string "Received ServerHelloDone\n";
+
   let KEX_S_DHE gy = ske.ske_kex_s in
   let gx, pms = CommonDH.dh_responder gy in
   let cke = {cke_kex_c = kex_c_of_dh_key gx} in
   let ckeb = clientKeyExchangeBytes sh.sh_protocol_version cke in
   IO.print_string "Sending ClientKeyExchange\n";
   let log = sendHSRecord tcp pv log ckeb in
+
   let ms = TLSPRF.prf (pv,cs) pms (utf8 "master secret") (ch.ch_client_random @| sh.sh_server_random)  48 in
   IO.print_string ("master secret:"^(Platform.Bytes.print_bytes ms)^"\n");
+
   let (ck,civ,sk,siv) = deriveKeys_TLS12_AES_GCM_128_SHA256 ms ch.ch_client_random sh.sh_server_random in
   IO.print_string ("client AES_GCM write key:"^(Platform.Bytes.print_bytes ck)^"\n");
   IO.print_string ("client AES_GCM salt: iv:"^(Platform.Bytes.print_bytes civ)^"\n");
@@ -228,14 +247,20 @@ let main host port =
   IO.print_string ("server AES_GCM salt:"^(Platform.Bytes.print_bytes siv)^"\n");
   let wr = encryptor_TLS12_AES_GCM_128_SHA256 ck civ in
   let rd = decryptor_TLS12_AES_GCM_128_SHA256 sk siv in
+
+
   IO.print_string "Sending ClientCCS\n";
   sendCCSRecord tcp pv;
+
   let cfin = {fin_vd = TLSPRF.verifyData (pv,cs) ms Client log} in 
   let cfinb = finishedBytes cfin in
   let efinb = encryptRecord_TLS12_AES_GCM_128_SHA256 wr Content.Handshake cfinb in
   IO.print_string "Sending ClientFinished\n";
+
   let log = sendHSRecord tcp pv log efinb in
+
   let _ = recvCCSRecord tcp pv in
+
   IO.print_string "Received ServerCCS\n";
   let Finished(sfin),log = recvEncHSRecord tcp pv kex log rd in
   IO.print_string "Received ServerFinished\n";
